{
 "cells": [
  {
   "cell_type": "markdown",
   "id": "64b70763",
   "metadata": {},
   "source": [
    "## Chapter 5:  Exercise 5.4\n",
    "\n",
    "Consider the truncated power series representation for cubic splines with $K$ interior knots. Let:\n",
    "\n",
    "$$\n",
    "f(X) = \\sum_{j=0}^{3} \\beta_j X^j + \\sum_{k=i}^{K} \\theta_k \\left( X - \\zeta_k\\right)^{3}_{+}\n",
    "$$\n",
    "\n",
    "**Part 1:** Prove that the natural boundary conditions for natural cubic splines (section 5.2.1) imply the following linear constraints on the coefficients:\n",
    "\n",
    "\\begin{align}\n",
    "& \\beta_2 = 0, \\quad \\sum_{k=1}^{K} \\theta_k = 0 \\\\\n",
    "& \\beta_3 = 0, \\quad \\sum_{k=1}^{K} \\zeta_k \\theta_k = 0\n",
    "\\end{align}\n",
    "\n",
    "**Part 2:** Hence derive the basis (5.4) and (5.5)\n",
    "\n",
    "---"
   ]
  },
  {
   "cell_type": "markdown",
   "id": "82a9904e",
   "metadata": {},
   "source": [
    "### Part 1\n",
    "\n",
    "Natural cubic splines constraints the function to be linear beyond the boundary knots, i.e $f''(X) = 0$ and $f'''(x) = 0$ for $X <= \\zeta_1$ and $X >= \\zeta_K$\n",
    "\n",
    "\\begin{align}\n",
    "& f'(X) = \\beta_1 + \\beta_2 X + 3 \\beta_3 X^2 + \\sum_{k=1}^{K} 3 \\theta_k (X - \\zeta_k)^2 \\tag{1} \\\\ \n",
    "& f''(X) = \\beta_2 + 6 \\beta_3 X + \\sum_{k=1}^{K} 6 \\theta_k (X - \\zeta_k) \\tag{2} \\\\\n",
    "& f'''(X) =  6 \\beta_3 + \\sum_{k=1}^{K} 6 \\theta_k \\tag{3}\n",
    "\\end{align}\n",
    "\n",
    "Since (2), for $X <= \\zeta_1$ is equal to zero the only possible solution is that $\\beta_2 = 0$ and $\\beta_3 = 0$. Replacing $\\beta_3 = 0$ in (3) implies that $\\sum_{k=1}^{K} \\theta_k = 0$. Finally replacing $\\beta_2$ and $\\beta_3$ in (2) for $X >= \\zeta_K$:\n",
    "\n",
    "\\begin{align}\n",
    "& 0 = \\sum_{k=1}^{K} \\theta_k (X - \\zeta_k) \\\\\n",
    "& 0 = X \\sum_{k=1}^{K} \\theta_k - \\sum_{k=1}^{K} \\theta_k \\zeta_k \\\\\n",
    "& 0 = \\sum_{k=1}^{K} \\theta_k \\zeta_k \\\\\n",
    "\\end{align}\n",
    "\n",
    "In conclusion: $\\beta_2, \\beta_3, \\sum_{k=1}^{K}\\theta_k, \\sum_{k=1}^{K}\\theta_k \\zeta_k$ are all equal to 0.\n",
    "\n",
    "---"
   ]
  },
  {
   "cell_type": "markdown",
   "id": "1e062757",
   "metadata": {},
   "source": [
    "### Part 2\n",
    "\n",
    "Now that $\\beta_2$ and $\\beta_3$ are equal to 0, $f(X) = \\beta_0 + \\beta_1 + \\sum_{k=1}^{K}\\theta_k \\left( X - \\zeta_k \\right)^{3}_{+}$. By the results from part 1 we can free two parameters, say $\\theta_K$ and $\\theta_{K-1}$\n",
    "\n",
    "$$\n",
    "0 = \\sum_{k=1}^{K} \\theta_k \\Rightarrow \\theta_K = - \\sum_{k=1}^{K-1} \\theta_k \\tag{4}\n",
    "$$\n",
    "\n",
    "Combining results from part 1:\n",
    "\n",
    "\\begin{align}\n",
    "\\left(\\sum_{k=1}^{K} \\theta_k \\right) \\zeta_K - \\sum_{k=1}^{K}\\theta_k \\zeta_k  & = 0 \\\\\n",
    "\\sum_{k=1}^{K} \\theta_k (\\zeta_K - \\zeta_k)  & = 0 \\\\\n",
    "\\sum_{k=1}^{K-1} \\theta_k (\\zeta_K - \\zeta_k)  & = 0\n",
    "\\end{align}\n",
    "\n",
    "Isolationg $\\theta_{K-1}$\n",
    "\n",
    "$$\n",
    "\\theta_{K-1} = - \\sum_{k=1}^{K-2} \\frac{\\theta_k (\\zeta_K - \\zeta_k)}{\\zeta_K - \\zeta_{K-1}}\n",
    "$$\n",
    "\n",
    "Replacing $\\theta_K$ in $f$:\n",
    "\n",
    "\\begin{align}\n",
    "f(X) & = \\beta_0 + \\beta_1 X + \\sum_{k=1}^{K}\\theta_k \\left( X - \\zeta_k \\right)^{3}_{+} \\\\\n",
    "& = \\beta_0 + \\beta_1 X + \\sum_{k=1}^{K-1}\\theta_k \\left( X - \\zeta_k \\right)^{3}_{+} + \\theta_K(X - \\zeta_K)^{3}_{+} \\\\\n",
    "& = \\beta_0 + \\beta_1 X + \\sum_{k=1}^{K-1}\\theta_k \\left( X - \\zeta_k \\right)^{3}_{+} + \\sum_{k=1}^{K-1} \\theta_k (X - \\zeta_K)^{3}_{+} \\\\\n",
    " & = \\beta_0 + \\beta_1 X + \\sum_{k=1}^{K-1}\\theta_k \\left [\\left( X - \\zeta_k \\right)^{3}_{+} - \\left(X - \\zeta_K \\right)^{3}_{+} \\right]  \\\\\n",
    " & = \\beta_0 + \\beta_1 X + \\sum_{k=1}^{K-1}\\theta_k d_k(X) \\left(\\zeta_K - \\zeta_{k} \\right)\n",
    "\\end{align}\n",
    "\n",
    "\n",
    "Finally by replacing $\\theta_{K-1}$\n",
    "\n",
    "\\begin{align}\n",
    "f(X) & = \\beta_0 + \\beta_1 X + \\sum_{k=1}^{K-2}\\theta_k d_k(X) \\left(\\zeta_K - \\zeta_{k} \\right) + \\theta_{K-1} d_{K-1}(X) \\left(\\zeta_K - \\zeta_{K-1} \\right)\\\\\n",
    "& = \\beta_0 + \\beta_1 X + \\sum_{k=1}^{K-2}\\theta_k d_k(X) \\left(\\zeta_K - \\zeta_{k} \\right) -  \\sum_{k=1}^{K-2} \\frac{\\theta_k (\\zeta_K - \\zeta_k)}{\\zeta_K - \\zeta_{K-1}} d_{K-1}(X) \\left(\\zeta_K - \\zeta_{K-1} \\right) \\\\\n",
    "& = \\beta_0 + \\beta_1 X + \\sum_{k=1}^{K-2}\\theta_k \\left(\\zeta_K - \\zeta_{k} \\right) \\left( d_k(X) -  d_{K-1}(X) \\right) \\\\\n",
    "& = \\beta_0 + \\beta_1 X + \\sum_{k=1}^{K-2}\\theta_k \\left(\\zeta_K - \\zeta_{k} \\right) N_{k+2}(X)\n",
    "\\end{align}\n",
    "\n",
    "Since $(\\zeta_K - \\zeta_{k})$ do not depend on X, it is safe to define the new parameters $\\theta'_k := \\theta_k (\\zeta_K - \\zeta_{k})$ resulting in:\n",
    "\n",
    "$$\n",
    "f(X) = \\beta_0 + \\beta_1 X + \\sum_{k=1}^{K-2}\\theta'_k N_{k+2}(X)\n",
    "$$"
   ]
  }
 ],
 "metadata": {
  "kernelspec": {
   "display_name": "JC",
   "language": "python",
   "name": "universidad"
  },
  "language_info": {
   "codemirror_mode": {
    "name": "ipython",
    "version": 3
   },
   "file_extension": ".py",
   "mimetype": "text/x-python",
   "name": "python",
   "nbconvert_exporter": "python",
   "pygments_lexer": "ipython3",
   "version": "3.9.1"
  }
 },
 "nbformat": 4,
 "nbformat_minor": 5
}
